formal/ERIEC/RefModel.lean
@@ -1,2 +1,3 @@
 import ERIEC.RefModel.LargeCore
 import ERIEC.RefModel.LineageWitness
+import ERIEC.RefModel.CollapseTrace
